code complete on translating parsers and validators

src/frontend/Translate.fst
@@ -4,6 +4,63 @@ module A = Ast
 module T = Target
 open FStar.All
 
+let gen_ident : unit -> St ident =
+  let open FStar.ST in
+  let ctr : ref int = alloc 0 in
+  let next () =
+    let v = !ctr in
+    ctr := v + 1;
+    let id = Printf.sprintf "_x_%d" v in
+    with_dummy_range id
+  in
+  next
+
+let mk_lam (f:(A.ident -> ML 'a)) : ML (T.lam 'a) =
+  let x = gen_ident () in
+  x, f x
+
+let map_lam (x:T.lam 'a) (g: 'a -> ML 'b) : ML (T.lam 'b) =
+  fst x, g (snd x)
+
+let pk = ()
+
+let mk_parser k t p = T.({
+  p_kind = k;
+  p_typ = t;
+  p_parser = p
+})
+
+let unit_typ =
+    T.T_app (with_dummy_range "unit") []
+let unit_val =
+    T.Record (with_dummy_range "unit") []
+let unit_parser =
+    mk_parser pk unit_typ (T.Parse_return unit_val)
+let pair_typ t1 t2 =
+    T.T_app (with_dummy_range "tuple2") [Inl t1; Inl t2]
+let pair_value x y =
+    T.Record (with_dummy_range "tuple2")
+             [(with_dummy_range "fst", T.Identifier x);
+              (with_dummy_range "snd", T.Identifier y)]
+let pair_parser p1 p2 =
+    let open T in
+    let pt = pair_typ p1.p_typ p2.p_typ in
+    mk_parser pk pt (Parse_seq p1 p2)
+let dep_pair_typ t1 (t2:T.lam T.typ) : T.typ =
+    T.T_dep_pair t1 t2
+let dep_pair_value x y : T.expr =
+    T.Record (with_dummy_range "dtuple2")
+             [(with_dummy_range "fst", T.Identifier x);
+              (with_dummy_range "snd", T.Identifier y)]
+let dep_pair_parser p1 (p2:T.lam T.parser) =
+  let open T in
+  let x, p2 = p2 in
+  let t = T_dep_pair p1.p_typ (x, p2.p_typ) in
+  mk_parser pk t
+      (Parse_and_then
+        p1
+        (x, mk_parser pk t (Parse_map p2 (mk_lam (dep_pair_value x)))))
+
 let translate_op : A.op -> ML T.op = function
   | Eq -> T.Eq
   | And -> T.And
@@ -29,26 +86,19 @@ let translate_typ (t:A.typ) : ML T.typ =
   T.T_app hd (List.map (fun x -> Inr (translate_expr x)) args)
 
 let translate_typedef_name (tdn:A.typedef_names) params : ML T.typedef_name =
-  let params = List.map (fun (id, t) -> id, translate_typ t) params in
+  let params = List.map (fun (t, id) -> id, translate_typ t) params in
   tdn.typedef_name, params
 
 let make_enum_typ (t:T.typ) (ids:list ident) =
-  let refinement (x:A.ident) =
-    let x = T.Identifier x in
+  let refinement i =
+    let x = T.Identifier i in
     List.fold_right
       (fun y e -> T.App T.Or [T.App T.Eq [T.Identifier y; x]; e])
       ids
       (T.Constant (Bool false))
   in
-  T.T_refine t refinement
+  T.T_refine t (mk_lam refinement)
 
-let pk = ()
-
-let mk_parser k t p = T.({
-  p_kind = k;
-  p_typ = t;
-  p_parser = p
-})
 
 let rec parse_typ (t:T.typ) : ML T.parser =
   let open T in
@@ -68,6 +118,9 @@ let rec parse_typ (t:T.typ) : ML T.parser =
         cases
     in
     mk_parser pk t (T.Parse_cases head cases)
+
+  | T.T_dep_pair t1 (x, t2) ->
+    dep_pair_parser (parse_typ t1) (x, parse_typ t2)
 
 let pv p v = T.({
   v_parser = p;
@@ -103,7 +156,10 @@ let rec make_validator (p:T.parser) : ML T.validator =
     pv p (Validate_seq (make_validator p1) (make_validator p2))
 
   | Parse_and_then p1 k ->
-    pv p (Validate_and_read (make_validator p1) (make_reader p1.p_typ) (fun x -> make_validator (k x)))
+    pv p (Validate_and_read
+            (make_validator p1)
+            (make_reader p1.p_typ)
+            (map_lam k make_validator))
 
   | Parse_map p1 f ->
     pv p (Validate_map (make_validator p1) f)
@@ -117,13 +173,77 @@ let rec make_validator (p:T.parser) : ML T.validator =
   | Parse_cases hd cs ->
     pv p (Validate_cases hd (List.map (fun (e, p) -> e, make_validator p) cs))
 
-let nondep_group = nat & list struct_field
-let grouped_fields = list (either struct_field nondep_group)
-let maked_grouped_fields (fs:list A.field) : ML grouped_fields =
+// x:t1;
+// t2;
+// t3;
+// y:t4;
+// t5;
+// t6
+
+// (x <-- parse_t1 ;
+//  (parse_t2 ;;
+//   parse_t3 ;;
+//   (y <-- parse_t4;
+//     ((parse_t5 ;;
+//       parse_t6) `map` (fun x56 -> y, x56))))
+//  `map` (fun x_2_3_4_5_6 -> {x = x; y .... }))
+
+// let rec translate_grouped_fields
+//          (gfs:grouped_fields) =
+//   let translate_one_field sf =
+//       let t = translate_typ sf.field_typ in
+//       let t =
+//         match sf.field_array_opt with
+//         | None -> t
+//         | Some e ->
+//           let e = translate_expr e in
+//           T.T_app "lseq" [Inl t; Inr e]
+//       in
+//       let t =
+//         match sf.constraint with
+//         | None -> t
+//         | Some e ->
+//           T.T_refine t (fun x -> translate_expr e)
+//   in
+//   match gfs with
+//   | [] -> failwith "Empty fields"
+//   | Inl sf::tl ->
+
+
+let translate_struct_field (sf:A.struct_field) : ML T.struct_field =
+    let t = translate_typ sf.field_type in
+    let t =
+        match sf.field_array_opt with
+        | None -> t
+        | Some e ->
+          let e = translate_expr e in
+          T.T_app (with_range "lseq" sf.field_type.range) [Inl t; Inr e]
+    in
+    let t =
+      match sf.field_constraint with
+      | None -> t
+      | Some e ->
+        T.T_refine t (sf.field_ident, translate_expr e)
+    in
+    T.({sf_dependence=sf.field_dependence;
+        sf_ident=sf.field_ident;
+        sf_typ=t})
+
+let translate_field (f:A.field) : ML T.field =
+  match f.v with
+  | FieldComment s ->
+    T.FieldComment s
+  | Field sf ->
+    T.Field (translate_struct_field sf)
+
+let nondep_group = nat & list T.struct_field
+let grouped_fields = list (either T.struct_field nondep_group)
+let make_grouped_fields (fs:list T.field) : ML grouped_fields =
+  let open T in
   let sfs =
     List.filter_map
       (fun f ->
-        match f.v with
+        match f with
         | Field sf -> Some sf
         | _ -> None)
       fs
@@ -140,7 +260,7 @@ let maked_grouped_fields (fs:list A.field) : ML grouped_fields =
           (sf:struct_field)
           (out, run)
     : grouped_fields & nondep_group
-    = if sf.field_dependence
+    = if sf.sf_dependence
       then Inl sf :: add_run (out, run), (0, [])
       else out, extend_run sf run
   in
@@ -163,35 +283,78 @@ let maked_grouped_fields (fs:list A.field) : ML grouped_fields =
 //     ((parse_t5 ;;
 //       parse_t6) `map` (fun x56 -> y, x56))))
 //  `map` (fun x_2_3_4_5_6 -> {x = x; y .... }))
+let parse_grouped_fields (gfs:grouped_fields)
+  : ML T.parser
+  = let open T in
+    let rec aux (gfs:grouped_fields) : ML parser =
+      match gfs with
+      | [] ->
+        unit_parser
 
-let rec translate_grouped_fields
-         (gfs:grouped_fields) =
-  let translate_one_field sf =
-      let t = translate_typ sf.field_typ in
-      let t =
-        match sf.field_array_opt with
-        | None -> t
-        | Some e ->
-          let e = translate_expr e in
-          T.T_app "lseq" [Inl t; Inr e]
-      in
-      let t =
-        match sf.constraint with
-        | None -> t
-        | Some e ->
-          T.T_refine t (fun x -> translate_expr e)
+      | Inl sf::gfs ->
+        dep_pair_parser (parse_typ sf.sf_typ) (sf.sf_ident, aux gfs)
+
+      | Inr (_, gf)::gfs ->
+        List.fold_right
+          (fun (sf:struct_field) (p_tl:parser) ->
+            pair_parser (parse_typ sf.sf_typ) p_tl)
+          gf
+          (aux gfs)
+    in
+    aux gfs
+
+let parse_fields (tdn:T.typedef_name) (fs:list T.field) =
+  let open T in
+  let td_name, td_params = tdn in
+  let gfs = make_grouped_fields fs in
+  let p = parse_grouped_fields gfs in
+  let dfst (e:T.expr) = App (Ext "dfst") [e] in
+  let dsnd (e:T.expr) = App (Ext "dsnd") [e] in
+  let fst (e:T.expr) = App (Ext "fst") [e] in
+  let snd (e:T.expr) = App (Ext "snd") [e] in
+  let rec make_non_dep_record_fields (e:T.expr) (fs:list struct_field)
+    : Tot  (list (A.ident * T.expr)) (decreases fs) =
+    match fs with
+    | [] -> []
+    | [hd] -> [hd.sf_ident, e]
+    | hd::tl -> (hd.sf_ident, fst e) :: make_non_dep_record_fields (snd e) tl
   in
-  match gfs with
-  | [] -> failwith "Empty fields"
-  | Inl sf::tl ->
+  let rec make_record_fields (e:T.expr) (gfs:grouped_fields)
+    : Tot  (list (A.ident * T.expr)) (decreases gfs) =
+    match gfs with
+    | [] -> []
+    | Inl hd::gfs ->
+      (hd.sf_ident, dfst e) :: make_record_fields (dsnd e) gfs
+    | Inr (_,gf)::gfs ->
+      let tl = make_record_fields (snd e) gfs in
+      let head = make_non_dep_record_fields (fst e) gf in
+      head @ tl
+  in
+  let make_record (x:A.ident) =
+    let fields = make_record_fields (T.Identifier x) gfs in
+    Record td_name fields
+  in
+  let t = T_app td_name (List.map (fun (x, _) -> Inr (T.Identifier x)) td_params) in
+  mk_parser pk t (Parse_map p (mk_lam make_record))
 
-
-
-
-// let translate_fields (fs:list A.field) =
-//   let gfs
-
-//   ()
+let translate_switch_case_type (sw:Ast.switch_case) =
+  let sc, cases = sw in
+  let sc = translate_expr sc in
+  let translate_case ef : ML (list T.case) =
+    let e, f = ef in
+    let pat = translate_expr e in
+    match f.v with
+    | FieldComment _ -> []
+    | Field sf ->
+      let sf = translate_struct_field sf in
+      let open T in
+      [{
+        pattern = pat;
+        branch = sf.sf_typ
+       }]
+  in
+  let cases = List.collect translate_case cases in
+  T.T_match sc cases
 
 let translate_decl (d:A.decl) : ML T.decl =
   match d.v with
@@ -202,48 +365,48 @@ let translate_decl (d:A.decl) : ML T.decl =
   | Enum t i ids ->
     let tdn = {
         typedef_name = i;
-        typedef_abbrev = "";
-        typedef_ptr_abbrev = "";
+        typedef_abbrev = with_dummy_range "";
+        typedef_ptr_abbrev = with_dummy_range "";
       }
     in
-    let typ = translate_typ typ in
-    let typedef_name = translate_typedef_name tdn [] in
+    let typ = translate_typ t in
+    let tdn = translate_typedef_name tdn [] in
     let refined_typ = make_enum_typ typ ids in
-    let parser = parse_typ refined_typ in
+    let p = parse_typ refined_typ in
     let open T in
     Type_decl (
       {
-        decl_name = typedef_name;
+        decl_name = tdn;
         decl_typ = TD_abbrev refined_typ;
-        decl_parser = parser;
-        decl_validator = make_validator parser;
+        decl_parser = p;
+        decl_validator = make_validator p;
       }
     )
 
   | Record tdn params ast_fields ->
-    let typedef_name = translate_typedef_name tdn params in
-    let fields = translate_fields ast_fields in
-    let parser = parse_fields ast_fields in
+    let tdn = translate_typedef_name tdn params in
+    let fields = List.map translate_field ast_fields in
+    let p = parse_fields tdn fields in
     let open T in
     Type_decl (
       {
-        decl_name = typedef_name;
+        decl_name = tdn;
         decl_typ = TD_struct fields;
-        decl_parser = parser;
-        decl_validator = make_validator parser
+        decl_parser = p;
+        decl_validator = make_validator p
       }
     )
 
   | CaseType tdn params switch_case ->
-    let typedef_name = translate_typedef_name tdn params in
-    let typ = translate_switch_case_type typ in
-    let parser = parse_cases typ in
+    let tdn = translate_typedef_name tdn params in
+    let t = translate_switch_case_type switch_case in
+    let p = parse_typ t in
     let open T in
     Type_decl (
       {
-        decl_name = typedef_name;
-        decl_typ = TD_abbrev typ;
-        decl_parser = parser;
-        decl_validator = make_validator parser
+        decl_name = tdn;
+        decl_typ = TD_abbrev t;
+        decl_parser = p;
+        decl_validator = make_validator p
       }
     )
