src/frontend/Target.fst
@@ -15,7 +15,7 @@ type op =
   | GT
   | LE
   | GE
-
+  | Ext of string
 /// Same as A.expr, but with `This` removed
 noeq
 type expr =
@@ -24,12 +24,15 @@ type expr =
   | App        : hd:op -> args:list expr -> expr
   | Record     : type_name:A.ident -> list (A.ident * expr) -> expr
 
+type lam a = A.ident & a
+
 (* A subset of F* types that the translation targets *)
 noeq
 type typ =
-  | T_app   : hd:A.ident -> args:list index -> typ
-  | T_refine: base:typ -> refinement:(A.ident -> ML expr) -> typ
-  | T_match : scrutinee:expr -> list case -> typ
+  | T_app      : hd:A.ident -> args:list index -> typ
+  | T_dep_pair : dfst:typ -> dsnd:lam typ -> typ
+  | T_refine   : base:typ -> refinement:lam expr -> typ
+  | T_match    : scrutinee:expr -> list case -> typ
 
 (* One arm of a match *)
 and case = {
@@ -43,11 +46,22 @@ and case = {
 and index = either typ expr
 
 type param = A.ident & typ
-type field = A.ident & typ
+noeq
+type struct_field = {
+  sf_dependence: bool;
+  sf_ident: A.ident;
+  sf_typ: typ
+}
+noeq
+type field =
+  | Field : struct_field -> field
+  | FieldComment : string -> field
+type comment = string
+
 noeq
 type typedef_body =
   | TD_abbrev : typ -> typedef_body
-  | TD_struct : list (bool * field) -> typedef_body
+  | TD_struct : list field  -> typedef_body
 
 type typedef_name = A.ident & list param
 type typedef = typedef_name & typedef_body
@@ -61,9 +75,9 @@ type parser' =
   | Parse_app       : hd:A.ident -> args:list index -> parser'
   | Parse_return    : v:expr -> parser'
   | Parse_seq       : p:parser -> q:parser -> parser'
-  | Parse_and_then  : p:parser -> k:(A.ident -> ML parser) -> parser'
-  | Parse_map       : p:parser -> f:(A.ident -> ML expr) -> parser'
-  | Parse_filter    : p:parser -> f:(A.ident -> ML expr) -> parser'
+  | Parse_and_then  : p:parser -> k:lam parser -> parser'
+  | Parse_map       : p:parser -> f:lam expr -> parser'
+  | Parse_filter    : p:parser -> f:lam expr -> parser'
   | Parse_with_kind : p:parser -> k:parser_kind -> parser'
   | Parse_cases     : e:expr -> list (expr * parser) -> parser'
 
@@ -78,17 +92,17 @@ type reader =
   | Read_u8
   | Read_u16
   | Read_u32
-  | Read_filter : r:reader -> f:(A.ident -> ML expr) -> reader
+  | Read_filter : r:reader -> f:lam expr -> reader
 
 noeq
 type validator' =
   | Validate_app      : hd:A.ident -> args:list index -> validator'
   | Validate_return   : validator'
   | Validate_seq      : v1:validator -> v2:validator -> validator'
-  | Validate_and_read : v:validator -> r:reader -> k:(A.ident -> ML validator) -> validator'
-  | Validate_map      : p:validator -> f:(A.ident -> ML expr) -> validator'
-  | Validate_filter   : v:validator -> r:reader -> f:(A.ident -> ML expr) -> validator'
-  | Validate_filter_and_read : v:validator -> r:reader -> f:(A.ident -> ML expr) -> k:(A.ident -> ML validator) -> validator'
+  | Validate_and_read : v:validator -> r:reader -> k:lam validator -> validator'
+  | Validate_map      : p:validator -> f:lam expr -> validator'
+  | Validate_filter   : v:validator -> r:reader -> f:lam expr -> validator'
+  | Validate_filter_and_read : v:validator -> r:reader -> f:lam expr -> k:lam validator -> validator'
   | Validate_with_kind : v:validator -> validator'
   | Validate_cases    : e:expr -> list (expr * validator) -> validator'
 
